NumLean/Data/Array/TensorOps.lean
@@ -14,8 +14,8 @@ def fillTensorSlice {r} (shape : Shape r)
     (dst : Array K) (dstLayout : Layout shape Nat) (x : K) : Array K :=
   Id.run do
     let mut dst := dst
-    for jt in rowMajorIter shape do
-      let di := dstLayout.eval jt.1
+    for (_linear, jt) in rowMajorIter shape do
+      let di := dstLayout.eval jt
       if h : di < dst.size then
         dst := dst.set di x h
     return dst
@@ -26,9 +26,9 @@ def copyTensorSlice {r} (shape : Shape r)
     (dst : Array K) (dstLayout : Layout shape Nat) : Array K :=
   Id.run do
     let mut dst := dst
-    for jt in rowMajorIter shape do
-      let si := srcLayout.eval jt.1
-      let di := dstLayout.eval jt.1
+    for (_linear, jt) in rowMajorIter shape do
+      let si := srcLayout.eval jt
+      let di := dstLayout.eval jt
       if hs : si < src.size then
         if hd : di < dst.size then
           dst := dst.set di src[si] hd
@@ -39,9 +39,8 @@ def extractTensorSlice [Inhabited K] {r} (shape : Shape r)
     (src : Array K) (srcLayout : Layout shape Nat) : Array K :=
   Id.run do
     let mut out := Array.replicate shape.size default
-    for jt in rowMajorIter shape do
-      let si := srcLayout.eval jt.1
-      let oi := (equivFin shape jt).1
+    for (oi, jt) in rowMajorIter shape do
+      let si := srcLayout.eval jt
       if hs : si < src.size then
         if ho : oi < out.size then
           out := out.set oi src[si] ho
